src/parser/FStar.Parser.Const.fst
@@ -38,7 +38,6 @@ let fstar_ns_lid          = p2l ["FStar"]
 (* Primitive types *)
 let bool_lid         = pconst "bool"
 let unit_lid         = pconst "unit"
-let unit_as_type_lid = psconst "unit_as_type"
 let squash_lid       = pconst "squash"
 let auto_squash_lid  = pconst "auto_squash"
 let string_lid       = pconst "string"
@@ -123,8 +122,8 @@ let assume_lid            = pconst  "_assume"
 let assert_lid            = pconst  "_assert"
 let pure_wp_lid           = pconst "pure_wp"
 let trivial_pure_post_lid = psconst "trivial_pure_post"
-let pure_assert_wp_lid    = pconst "pure_assert_wp"
-let pure_assume_wp_lid    = pconst "pure_assume_wp"
+let pure_assert_wp_lid    = pconst "pure_assert_wp0"
+let pure_assume_wp_lid    = pconst "pure_assume_wp0"
 let assert_norm_lid       = p2l ["FStar"; "Pervasives"; "assert_norm"]
 (* list_append_lid is needed to desugar @ in the compiler *)
 let list_append_lid       = p2l ["FStar"; "List"; "append"]
